\documentclass{article}%book，report，letter

\usepackage{ctex}
\usepackage{fontspec}
%\usepackage{color}
%\usepackage{graphicx} %use graph format
%\usepackage{subfigure}
%\usepackage{epstopdf} %eps图片
\usepackage{amsmath}  %字体加粗
%\usepackage{math}
\usepackage{amsthm}
\usepackage{amssymb} %因为所以符号
%\usepackage{caption}
%\captionsetup[table]{labelsep=space}

%制作页眉页脚
\usepackage{fancyhdr}
\pagestyle{fancy}
\lhead{第八周作业}
\chead{微分方程数值解法}
\rhead{桑明达 15300180062}
\lfoot{}
\cfoot{\thepage}
\rfoot{}
\renewcommand{\headrulewidth}{0.4pt}
\renewcommand{\footrulewidth}{0.4pt}

%标题
\author{names}
\title{\heiti 微分方程数值解法\\ [2ex] \begin{large} 第八周作业 \end{large}}
\author{\kaishu 桑明达 15300180062}
\date{\today}

% 正文区
\begin{document}
\maketitle

%\newpage

\section{P136 附加 求Green函数}

\begin{proof}

	当$ G\left ( 0 \right )=0;G'\left ( 1 \right )=0$,有

\begin{align*}
	G\left ( x;x_0 \right )=\left\{\begin{matrix}
x &0< x<x_0 \\
x_0 &x_0<x<1
\end{matrix}\right.
\end{align*}

\end{proof}


\section{P136 1 求函数u}

\begin{proof}

	解方程，得$$ u=\frac{1}{k^2}+C_1 e^{kix}+C_2 e^{-kix} $$

	代入	$ u\left ( 0 \right )=0;u\left ( 1 \right )=0$，得$$ C_1=\frac{e^{-ki}-1}{k^2\left ( e^{ki}-e^{-ki} \right )},C_2=\frac{1-e^{ki}}{k^2\left ( e^{ki}-e^{-ki} \right )} $$

	此时，$$ Lu=-u_{xx}-k^2u=-1<0 $$

	而 $$ u_{x}=kiC_1\left (e^{kix} -e^{ki\left ( 1-x \right )} \right ) $$

	即存在极值$$ u\left ( 0.5 \right )=\frac{1}{k^2}>0=u\left ( 0 \right )=u\left ( 1 \right ) $$

	不符合极值原理。

\end{proof}

\section{P136 3 验证函数u(x)}

\begin{proof}

	(1)对于初值

\begin{align*}
	u\left ( 0 \right )&=\int_{0}^{1}G\left ( 0;x_0 \right )f\left ( x_0 \right )\mathrm{d}x_0=0 \\
	u\left ( 1 \right )&=\int_{0}^{1}G\left ( 1;x_0 \right )f\left ( x_0 \right )\mathrm{d}x_0=0 \\
\end{align*}

(2)对于 $\forall x\in\left ( 0,1 \right )$,有

\begin{align*}
		u\left ( x \right )=&\int_{x}^{1}G\left ( x;x_0 \right )f\left ( x_0 \right )\mathrm{d}x_0+\int_{0}^{x}G\left ( x;x_0 \right )f\left ( x_0 \right )\mathrm{d}x_0\\
	=&\int_{x}^{1}x\left ( 1-x_0 \right )f\left ( x_0 \right )\mathrm{d}x_0+\int_{0}^{x}x_0\left ( 1-x \right )f\left ( x_0 \right )\mathrm{d}x_0\\
	\therefore u_x=&-\left ( 1-x \right )xf\left ( x \right )+\int_{x}^{1}\left ( 1-x_0 \right )f\left ( x_0 \right )\mathrm{d}x_0 \\
	&+x\left ( 1-x \right )f\left ( x \right )+\int_{0}^{x}x_0\left ( -1 \right ) f\left ( x_0 \right )\mathrm{d}x_0\\
	\therefore u_{xx}=&-\left ( 1-x \right )f\left ( x \right )+\left ( -x \right )f\left ( x \right )\\
	=&-f\left ( x \right )\\
\end{align*}
	即证。
\end{proof}

\end{document}
